open import Core
open import Data.Nat using (โ) renaming (_โ_ to _โ-nat_)
open import Data.Product using (_ร_; _,_; projโ)
open import Relation.Nullary using (Dec; yes; no; _ร-dec_) renaming (mapโฒ to map-dec)

module Eq where
  import Relation.Binary.PropositionalEquality as Eq
  open Eq public using (_โก_; refl; cong)

  DecEq : โ (T : Set) โ Set
  DecEq T = (l : T) โ (r : T) โ Dec (l โก r)

  instance
    DecEqNat : DecEq โ
    DecEqNat l r = l โ-nat r

  _โ_ : {T : Set} โฆ DecEqT : DecEq T โฆ โ (l : T) โ (r : T) โ Dec (l โก r)
  _โ_ โฆ DecEqT โฆ = DecEqT

  _โ-act_ : (aโ : Act) โ (aแตฃ : Act) โ Dec (aโ โก aแตฃ)
  โณ โ-act โณ = yes refl
  โณ โ-act โฅ = no (ฮป ())
  โฅ โ-act โณ = no (ฮป ())
  โฅ โ-act โฅ = yes refl

  instance
    DecEqAct : DecEq Act
    DecEqAct = _โ-act_

  _โ-gas_ : (gโ : Gas) โ (gแตฃ : Gas) โ Dec (gโ โก gแตฃ)
  ๐ โ-gas ๐ = yes refl
  ๐ โ-gas โ = no (ฮป ())
  โ โ-gas ๐ = no (ฮป ())
  โ โ-gas โ = yes refl

  instance
    DecEqGas : DecEq Gas
    DecEqGas = _โ-gas_

  _โ-exp_ : (eโ : Exp) โ (eแตฃ : Exp) โ Dec (eโ โก eแตฃ)
  _โ-pat_ : (pโ : Pat) โ (pแตฃ : Pat) โ Dec (pโ โก pแตฃ)

  -- instance
  --   DecEqProduct : โ {A B} โฆ DecEqA : DecEq A โฆ โฆ DecEqB : DecEq B โฆ โ DecEq (A ร B)
  --   DecEq.eq DecEqProduct (aโ , aแตฃ) (bโ , bแตฃ) with (aโ โ bโ) ร-dec (aแตฃ โ bแตฃ)
  --   DecEq.eq DecEqProduct (aโ , aแตฃ) (aโ , aแตฃ) | yes (refl , refl) = yes refl
  --   DecEq.eq DecEqProduct (aโ , aแตฃ) (bโ , bแตฃ) | no aโขb = no ฮป { refl โ aโขb (refl , refl) }

  (` x) โ-exp (` y) with x โ-nat y
  (` x) โ-exp (` y) | yes refl = yes refl
  (` x) โ-exp (` y) | no xโขy = no ฮป { refl โ xโขy refl }
  (` x) โ-exp (ฦ e) = no (ฮป ())
  (` x) โ-exp (l ยท r) = no (ฮป ())
  (` x) โ-exp (# n) = no (ฮป ())
  (` x) โ-exp (l + r) = no (ฮป ())
  (` x) โ-exp ฯ f e = no (ฮป ())
  (` x) โ-exp ฮด r e = no (ฮป ())
  (ฦ e) โ-exp (` x) = no (ฮป ())
  (ฦ l) โ-exp (ฦ r) with l โ-exp r
  (ฦ l) โ-exp (ฦ r) | yes refl = yes refl
  (ฦ l) โ-exp (ฦ r) | no lโขr = no ฮป { refl โ lโขr refl }
  (ฦ e) โ-exp (l ยท r) = no (ฮป ())
  (ฦ e) โ-exp (# n) = no (ฮป ())
  (ฦ e) โ-exp (l + r) = no (ฮป ())
  (ฦ _) โ-exp ฯ f e = no (ฮป ())
  (ฦ _) โ-exp ฮด r e = no (ฮป ())
  (lโ ยท lแตฃ) โ-exp (` x) = no (ฮป ())
  (lโ ยท lแตฃ) โ-exp (ฦ e) = no (ฮป ())
  (lโ ยท lแตฃ) โ-exp (rโ ยท rแตฃ) with (lโ โ-exp rโ) ร-dec (lแตฃ โ-exp rแตฃ)
  (lโ ยท lแตฃ) โ-exp (lโ ยท lแตฃ) | yes (refl , refl) = yes refl
  (lโ ยท lแตฃ) โ-exp (rโ ยท rแตฃ) | no lโขr = no ฮป { refl โ lโขr (refl , refl) }
  (lโ ยท lแตฃ) โ-exp (# n) = no (ฮป ())
  (lโ ยท lแตฃ) โ-exp (rโ + rแตฃ) = no (ฮป ())
  (lโ ยท lแตฃ) โ-exp ฯ f e = no (ฮป ())
  (lโ ยท lแตฃ) โ-exp ฮด r e = no (ฮป ())
  (# n) โ-exp (` x) = no (ฮป ())
  (# n) โ-exp (ฦ r) = no (ฮป ())
  (# n) โ-exp (r ยท rโ) = no (ฮป ())
  (# n) โ-exp (# m) with n โ-nat m
  (# n) โ-exp (# m) | yes refl = yes refl
  (# n) โ-exp (# m) | no nโขm = no ฮป { refl โ nโขm refl }
  (# n) โ-exp (r + rโ) = no (ฮป ())
  (# n) โ-exp ฯ f r = no (ฮป ())
  (# n) โ-exp ฮด r rโ = no (ฮป ())
  (lโ + lแตฃ) โ-exp (` x) = no (ฮป ())
  (lโ + lแตฃ) โ-exp (ฦ e) = no (ฮป ())
  (lโ + lแตฃ) โ-exp (rโ ยท rแตฃ) = no (ฮป ())
  (lโ + lแตฃ) โ-exp (# n) = no (ฮป ())
  (lโ + lแตฃ) โ-exp (rโ + rแตฃ) with (lโ โ-exp rโ) ร-dec (lแตฃ โ-exp rแตฃ)
  (lโ + lแตฃ) โ-exp (lโ + lแตฃ) | yes (refl , refl) = yes refl
  (lโ + lแตฃ) โ-exp (rโ + rแตฃ) | no lโขr = no ฮป { refl โ lโขr (refl , refl) }
  (lโ + lแตฃ) โ-exp ฯ f e = no (ฮป ())
  (lโ + lแตฃ) โ-exp ฮด r e = no (ฮป ())
  ฯ f l โ-exp (` x) = no (ฮป ())
  ฯ f l โ-exp (ฦ r) = no (ฮป ())
  ฯ f l โ-exp (r ยท rโ) = no (ฮป ())
  ฯ f l โ-exp (# n) = no (ฮป ())
  ฯ f l โ-exp (r + rโ) = no (ฮป ())
  ฯ fโ eโ โ-exp ฯ fแตฃ eแตฃ with ({!!}) ร-dec (eโ โ-exp eแตฃ)
  ฯ fโ eโ โ-exp ฯ fแตฃ eแตฃ | yes (x , refl) = yes x
  ฯ fโ eโ โ-exp ฯ fแตฃ eแตฃ | no lโขr = no ฮป { refl โ lโขr (refl , refl) }
  ฯ f l โ-exp ฮด r rโ = no (ฮป ())
  ฮด r eโ โ-exp (` x) = no (ฮป ())
  ฮด r eโ โ-exp (ฦ eแตฃ) = no (ฮป ())
  ฮด r eโ โ-exp (eแตฃ ยท eแตฃโ) = no (ฮป ())
  ฮด r eโ โ-exp (# n) = no (ฮป ())
  ฮด r eโ โ-exp (eแตฃ + eแตฃโ) = no (ฮป ())
  ฮด r eโ โ-exp ฯ f eแตฃ = no (ฮป ())
  ฮด rโ eโ โ-exp ฮด rแตฃ eแตฃ with ({!!}) ร-dec (eโ โ-exp eแตฃ)
  ฮด rโ eโ โ-exp ฮด rแตฃ eแตฃ | yes (x , refl) = yes {!!}
  ฮด rโ eโ โ-exp ฮด rแตฃ eแตฃ | no lโขr = no (ฮป { refl โ lโขr (refl , refl) })

  $e โ-pat $e = yes refl
  $e โ-pat $v = no (ฮป ())
  $e โ-pat (` x) = no (ฮป ())
  $e โ-pat (ฦ e) = no (ฮป ())
  $e โ-pat (pแตฃ ยท pแตฃโ) = no (ฮป ())
  $e โ-pat (# n) = no (ฮป ())
  $e โ-pat (pแตฃ + pแตฃโ) = no (ฮป ())
  $v โ-pat $e = no (ฮป ())
  $v โ-pat $v = yes refl
  $v โ-pat (` x) = no (ฮป ())
  $v โ-pat (ฦ e) = no (ฮป ())
  $v โ-pat (pแตฃ ยท pแตฃโ) = no (ฮป ())
  $v โ-pat (# n) = no (ฮป ())
  $v โ-pat (pแตฃ + pแตฃโ) = no (ฮป ())
  (` x) โ-pat $e = no (ฮป ())
  (` x) โ-pat $v = no (ฮป ())
  (` x) โ-pat (` y) with x โ-nat y
  (` x) โ-pat (` y) | yes refl = yes refl
  (` x) โ-pat (` y) | no xโขy = no (ฮป { refl โ xโขy refl })
  (` x) โ-pat (ฦ e) = no (ฮป ())
  (` x) โ-pat (pแตฃ ยท pแตฃโ) = no (ฮป ())
  (` x) โ-pat (# n) = no (ฮป ())
  (` x) โ-pat (pแตฃ + pแตฃโ) = no (ฮป ())
  (ฦ e) โ-pat $e = no (ฮป ())
  (ฦ e) โ-pat $v = no (ฮป ())
  (ฦ e) โ-pat (` x) = no (ฮป ())
  (ฦ eโ) โ-pat (ฦ eแตฃ) with eโ โ-exp eแตฃ
  (ฦ eโ) โ-pat (ฦ eแตฃ) | yes refl = yes refl
  (ฦ eโ) โ-pat (ฦ eแตฃ) | no lโขr = no ฮป { refl โ lโขr refl }
  (ฦ e) โ-pat (pแตฃ ยท pแตฃโ) = no (ฮป ())
  (ฦ e) โ-pat (# n) = no (ฮป ())
  (ฦ e) โ-pat (pแตฃ + pแตฃโ) = no (ฮป ())
  (pโ ยท pโโ) โ-pat $e = no (ฮป ())
  (pโ ยท pโโ) โ-pat $v = no (ฮป ())
  (pโ ยท pโโ) โ-pat (` x) = no (ฮป ())
  (pโ ยท pโโ) โ-pat (ฦ e) = no (ฮป ())
  (pโ ยท pโโ) โ-pat (pแตฃ ยท pแตฃโ) = {!!}
  (pโ ยท pโโ) โ-pat (# n) = no (ฮป ())
  (pโ ยท pโโ) โ-pat (pแตฃ + pแตฃโ) = no (ฮป ())
  (# n) โ-pat $e = no (ฮป ())
  (# n) โ-pat $v = no (ฮป ())
  (# n) โ-pat (` x) = no (ฮป ())
  (# n) โ-pat (ฦ e) = no (ฮป ())
  (# n) โ-pat (pแตฃ ยท pแตฃโ) = no (ฮป ())
  (# n) โ-pat (# m) with n โ-nat m
  (# n) โ-pat (# m) | yes refl = yes refl
  (# n) โ-pat (# m) | no nโขm = no ฮป { refl โ nโขm refl }
  (# n) โ-pat (pแตฃ + pแตฃโ) = no (ฮป ())
  (pโ + pโโ) โ-pat $e = no (ฮป ())
  (pโ + pโโ) โ-pat $v = no (ฮป ())
  (pโ + pโโ) โ-pat (` x) = no (ฮป ())
  (pโ + pโโ) โ-pat (ฦ e) = no (ฮป ())
  (pโ + pโโ) โ-pat (pแตฃ ยท pแตฃโ) = no (ฮป ())
  (pโ + pโโ) โ-pat (# n) = no (ฮป ())
  (pโ + pโโ) โ-pat (pแตฃ + pแตฃโ) = {!!}

  instance
    DecEqExp : DecEq Exp
    DecEqExp = _โ-exp_

  instance
    DecEqPat : DecEq Pat
    DecEqPat = _โ-pat_

